UnitProJ/expressOS/Fall2015/flycheck_INode-delRegion.dfy
@@ -635,15 +635,17 @@ nd in ndSet
 
 
 predicate delSeqHelperLemma(oldList:seq<INode>, oldFp:set<INode>, oldHdFp:set<INode>, hd:INode,newList:seq<INode>, newFp:set<INode>, newHdFp:set<INode>, fstNd:INode)
+	requires hd !in oldList && hd in oldFp && hd in oldHdFp;
 	requires forall nd:: nd in oldList && nd in oldFp ==> nd in oldHdFp - {hd};
 	requires oldList == [fstNd] + newList &&
-		oldFp == newFp + {fstNd} &&
-		oldHdFp == newHdFp + {fstNd};
+		oldFp - newFp == {fstNd} &&
+		oldHdFp - newHdFp == {fstNd};
 		
 	reads oldList, oldFp, oldHdFp, hd, newList, newFp, newHdFp;
 	ensures forall nd:: nd in newList && nd in newFp ==> nd in newHdFp - {hd};
 {true}
 
+/*
 method delSeqOfNd(ndList:seq<INode>)
 	requires valid();
 	requires null !in ndList;
@@ -666,13 +668,16 @@ method delSeqOfNd(ndList:seq<INode>)
 
 	assert footprint == old(footprint) - {ndList[0]};
 	assert head.footprint == old(head.footprint) - {ndList[0]};
+
+	assert delSeqHelperLemma(ndList, old(footprint), old(head.footprint), head, ndList[1..], footprint, head.footprint, ndList[0]);
+	
 delSeqOfNd(ndList[1..]);
 assert forall nd :: nd in ndList[1..] ==> nd !in footprint;
 assert forall nd :: nd in ndList ==> nd !in footprint;
 	}
 
 }
-
+*/
 
 
 }
